wn polish

theories/IntersectionTypes/Util/wn_facts.v
@@ -7,61 +7,112 @@ Require Import ssreflect ssrbool ssrfun.
 
 Set Default Proof Using "Type".
 
-#[local] Notation all P l := (fold_right and True (map P l)).
-
 Definition Arr (P Q : tm -> Prop) (M : tm) := forall N, P N -> Q (app M N).
 
-(*  forall N, (all (interp N) phi) -> interp (app M N) t *)
+#[local] Notation all P l := (fold_right and True (map P l)).
 
-Fixpoint interp (M : tm) (s : sty) : Prop :=
+Fixpoint interp (P : tm -> Prop) (M : tm) (s : sty) : Prop :=
   match s with
-  | atom a => wn M
-  | arr s phi t => Arr (fun N => (interp N s /\ all (interp N) phi)) (fun N => interp N t) M
+  | atom a => P M
+  | arr s phi t => Arr (fun N => (interp P N s /\ all (interp P N) phi)) (fun N => interp P N t) M
   end.
 
-Definition satis (Gamma : list ty) M t :=
-  forall sigma, (forall i s phi, nth_error Gamma i = Some (s, phi) -> interp (sigma i) s /\ (Forall (interp (sigma i)) phi)) ->
-  interp (subst sigma M) t.
+(* P-neutral term *)
+Inductive neutral (P : tm -> Prop) : tm -> Prop :=
+  | neutral_var x : neutral P (var x)
+  | neutral_app M N : neutral P M -> P N -> neutral P (app M N).
 
-Lemma Forall_all {X : Type} {P : X -> Prop} l : Forall P l <-> all P l.
+(* P-compatible head expansion *)
+Inductive head_exp (P : tm -> Prop) : tm -> tm -> Prop :=
+  | head_exp_lam M N : P N -> head_exp P (subst (scons N var) M) (app (lam M) N)
+  | head_exp_app M M' N : head_exp P M M' -> P N -> head_exp P (app M N) (app M' N).
+
+Record Saturated (Q P : tm -> Prop) :=
+  { Saturated_incl : forall M, P M -> Q M;
+    Saturated_neutral : forall M, neutral Q M -> P M }.
+
+Arguments Saturated_incl {Q P}.
+Arguments Saturated_neutral {Q P}.
+
+Record Admissible (P : tm -> Prop) :=
+  { Admissible_head_exp M N : head_exp P M N -> P M -> P N;
+    Admissible_neutral M : neutral P M -> P M;
+    Admissible_app_var M x : P (app M (var x)) -> P M }.
+
+Lemma Admissible_Saturated_interp {P} : Admissible P -> forall t, Saturated P (fun M => interp P M t).
 Proof.
-  elim: l. { done. }
-  move=> ?? IH. split.
-  - by move=> /Forall_cons_iff [? /IH].
-  - move=> [? ?]. constructor; first done. by apply /IH.
+  move=> HP. elim /sty_ind'.
+  { move=> x. constructor=> ?.
+    - done.
+    - by apply: (Admissible_neutral P HP). }
+  move=> s phi t IHs IHphi IHt. constructor=> M /= HM.
+  - have /HM : interp P (var 0) s /\ all (interp P (var 0)) phi.
+    { split. 
+      - apply: (Saturated_neutral IHs). by constructor.
+      - apply /Forall_all. apply: Forall_impl IHphi=> ?.
+        move=> /Saturated_neutral. apply. by constructor. }
+    move=> /(Saturated_incl IHt). by apply: (Admissible_app_var P HP).
+  - move=> N [+ _] => /(Saturated_incl IHs) ?.
+    apply: (Saturated_neutral IHt). by constructor.
 Qed.
 
-(* transforms a goal (A -> B) -> C into goals A and B -> C *)
-Lemma unnest : forall (A B C : Type), A -> (B -> C) -> (A -> B) -> C.
-Proof. auto. Qed.
-
-Inductive head_wn : tm -> Prop :=
-  | head_wn_var x : head_wn (var x)
-  | head_wn_app M N : head_wn M -> wn N -> head_wn (app M N).
-
-Lemma head_wnE M : head_wn M ->
-  match M with
-  | var _ => True
-  | lam _ => False
-  | app M1 M2 => head_wn M1 /\ wn M2
-  end.
-Proof. by case. Qed.
-
-Record Saturated (P : tm -> Prop) :=
-  { Saturated_wn : forall M, P M -> wn M;
-    Saturated_head_wn : forall M, head_wn M -> P M }.
-
-Lemma not_step_var x N : step (var x) N -> False.
-Proof. move E: (var x) => M HMN. by case: HMN E. Qed.
-
-Lemma head_wn_wn M : head_wn M -> wn M.
+Lemma interp_head_exp {P : tm -> Prop} {M N t} : Admissible P ->
+  head_exp P M N -> interp P M t -> interp P N t.
 Proof.
-  suff: head_wn M -> exists N, clos_refl_trans tm step M N /\ head_form N.
+  move=> HP. have HQ := Admissible_Saturated_interp HP. elim: t M N.
+  { move=> *. apply: (Admissible_head_exp _ HP); eassumption. }
+  move=> s ? phi t IH M N /= ? IH' N' [Hs Hphi].
+  apply: IH. { constructor; [|apply: (Saturated_incl (HQ _))]; eassumption. }
+  by apply: IH'.
+Qed.
+
+Definition satis (P : tm -> Prop) (Gamma : list ty) M t :=
+  forall sigma, (forall i s phi, nth_error Gamma i = Some (s, phi) -> interp P (sigma i) s /\ (Forall (interp P (sigma i)) phi)) ->
+  interp P (subst sigma M) t.
+
+Arguments satis P Gamma M !t /.
+
+Lemma satisI P Gamma M t : Admissible P -> type_assignment Gamma M t -> satis P Gamma M t.
+Proof.
+  move=> HP. have HQ := Admissible_Saturated_interp HP.
+  elim: M Gamma t.
+  - move=> a > /type_assignmentE [] s phi Ha H.
+    move=> sigma /(_ a _ _ Ha) [] /=.
+    case: H. { by move=> <-. }
+    by move=> + _ /Forall_forall {}H => /H.
+  - move=> ? IH1 ? IH2 ?? /type_assignmentE [] s phi /IH1 /= {}IH1 /IH2 {}IH3 Hphi.
+    move=> sigma Hsigma /=. apply: (IH1 sigma Hsigma). split.
+    { by apply: IH3. }
+    apply /Forall_all. apply: Forall_impl Hphi => ? /IH2. by apply.
+  - move=> ? IH1 ? [?|s phi t] /type_assignmentE; first done.
+    move=> /IH1 {}IH1 sigma HGamma /=.
+    move=> N [Hs Hphi]. apply: (interp_head_exp HP).
+    { apply: head_exp_lam. by apply: (Saturated_incl (HQ s)). }
+    rewrite simpl_tm. apply: IH1=> - [|i].
+    + move=> /= ?? [<- <-]. by split; [|apply /Forall_all].
+    + move=> ?? /HGamma => - [Hs' Hphi'] /=. by rewrite !simpl_tm.
+Qed.
+
+(* fundamental theorem for admissible predicates *)
+Theorem fundamental (P : tm -> Prop) Gamma M t : Admissible P ->
+  type_assignment Gamma M t -> P M.
+Proof.
+  move=> /[dup] HP /satisI /[apply] /(_ var). rewrite simpl_tm.
+  have HQ := Admissible_Saturated_interp HP.
+  move=> H. apply: (Saturated_incl (HQ _)).
+  apply: H=> i *. have : neutral P (var i) by constructor.
+  by split; [|apply /Forall_forall]=> *; apply: (Saturated_neutral (HQ _)).
+Qed.
+
+Module Admissible_wn.
+
+Lemma neutal_wn_wn M : neutral wn M -> wn M.
+Proof.
+  suff: neutral wn M -> exists N, clos_refl_trans tm step M N /\ head_form N.
   { move=> /[apply] - [?] [??]. by econstructor; [eassumption|constructor]. }
   elim. { move=> x. exists (var x). by split; [apply: rt_refl|constructor]. }
   move=> {}M N H1M [M'] [HMM' HM'] [N'] HNN' HN'.
   exists (app M' N'). split; [|by constructor].
-  (* many steps app L *)
   apply: (rt_trans _ _ _ (app M' N)).
   - elim: HMM'.
     + move=> > ?. apply: rt_step. by apply: stepAppL.
@@ -73,94 +124,21 @@ Proof.
     + move=> *. by apply: rt_trans; eassumption.
 Qed.
 
-Lemma step_lamE M N : step (lam M) N ->
-  exists M', N = lam M' /\ step M M'.
+Lemma head_exp_step M N : head_exp wn M N -> step N M.
 Proof.
-  move E: (lam M) => M0 H. case: H E => //.
-  move=> > ? [->]. by eexists.
+  elim. { move=> *. by apply: stepRed. }
+  move=> *. by apply: stepAppL.
 Qed.
 
-Lemma subst_as_ren M x : subst (scons (var x) var) M = ren (scons x id) M.
+Lemma step_wn M N : step M N -> wn N -> wn M.
 Proof.
-  rewrite ren_as_subst_tm /=. apply: ext_subst_tm. by case.
+  move=> ? [???]. econstructor; [|eassumption].
+  by apply: rt_trans; [apply: rt_step|]; eassumption.
 Qed.
 
-Lemma step_ren xi M N : step M N -> step (ren xi M) (ren xi N).
+Lemma head_exp_wn M N : head_exp wn M N -> wn M -> wn N.
 Proof.
-  move=> H. elim: H xi.
-  { move=> > /=.
-    evar (M1 : tm). evar (M2 : tm).
-    have := stepRed M1 M2. congr step.
-    rewrite /M1 /M2 !simpl_tm. apply: ext_subst_tm.
-    by case. }
-  all: by eauto using step with nocore.
-Qed.
-
-(* mutual induction on head_form, normal_form *)
-Scheme normal_form_ind' := Induction for normal_form Sort Prop
-  with head_form_ind' := Induction for head_form Sort Prop.
-
-Fact normal_form_ren xi M : 
-  normal_form M -> normal_form (ren xi M).
-Proof.
-  move=> H. move: H xi.
-  apply: (normal_form_ind' 
-    (fun M _ => forall xi, normal_form (ren xi M)) 
-    (fun M _ => forall xi, head_form (ren xi M)));
-      by eauto using normal_form, head_form.
-Qed.
-
-Fact normal_form_ren' xi M : 
-  normal_form (ren xi M) -> normal_form M.
-Proof.
-  move E: (ren xi M) => M' H. move: H xi M E.
-  apply: (normal_form_ind' 
-    (fun M' _ => forall xi M, ren xi M = M' -> normal_form M)
-    (fun M' _ => forall xi M, ren xi M = M' -> head_form M)).
-  - by eauto using normal_form, head_form.
-  - move=> > ? IH ? [] //= ? [?]. subst.
-    by eauto using normal_form, head_form.
-  - move=> ?? [] //= ? [?]. subst.
-    by eauto using normal_form, head_form.
-  - move=> > ????? [] //= ?? [??]. subst.
-    by eauto using normal_form, head_form.
-Qed.
-
-
-Lemma step_renE xi M N : step (ren xi M) N -> exists N', N = ren xi N' /\ step M N'.
-Proof.
-  move E: (ren xi M) => M' H. elim: H xi M E.
-  - move=> ??? [] //.
-    move=> [] // ?? /= [<- <-]. eexists.
-    split; first last. { by apply: stepRed. }
-    rewrite !simpl_tm. apply: ext_subst_tm.
-    by case.
-  - move=> > ? IH ? [] //= ? [?]. subst.
-    have [? [? ?]] := IH _ _ erefl. subst.
-    eexists.
-    split; first last. { apply: stepLam. eassumption. }
-    done.
-  - move=> > ? IH ? [] //= ?? [??]. subst.
-    have [? [? ?]] := IH _ _ erefl. subst.
-    eexists.
-    split; first last. { apply: stepAppL. eassumption. }
-    done.
-  - move=> > ? IH ? [] //= ?? [??]. subst.
-    have [? [? ?]] := IH _ _ erefl. subst.
-    eexists.
-    split; first last. { apply: stepAppR. eassumption. }
-    done.
-Qed.
-
-Lemma steps_renE xi M N : clos_refl_trans tm step (ren xi M) N -> exists N', N = ren xi N' /\ clos_refl_trans tm step M N'.
-Proof.
-  move E: (ren xi M) => M' /clos_rt_rt1n_iff H.
-  elim: H xi M E.
-  { move=> > <-. eexists. split;[done|]. by apply: rt_refl. }
-  move=> > +++ > ?. subst. move=> /step_renE [?] [->] ? _.
-  move=> /(_ _ _ erefl) [?] [->] ?.
-  eexists. split; [done|].
-  apply: rt_trans; [apply: rt_step|]; eassumption.
+  by move=> /head_exp_step /step_wn.
 Qed.
 
 Lemma wn_ren xi M : wn (ren xi M) -> wn M.
@@ -174,13 +152,7 @@ Proof.
   elim: HMN; by eauto using clos_refl_trans, step with nocore.
 Qed.
 
-Lemma step_wn M N : step M N -> wn N -> wn M.
-Proof.
-  move=> ? [???]. econstructor; [|eassumption].
-  by apply: rt_trans; [apply: rt_step|]; eassumption.
-Qed.
-
-Lemma wn_app_var x M : wn (app M (var x)) -> wn M.
+Lemma wn_app_var M x : wn (app M (var x)) -> wn M.
 Proof.
   case=> N /clos_rt_rt1n_iff.
   move E: (app M (var x)) => M' H. elim: H M E.
@@ -199,133 +171,18 @@ Proof.
     by move=> /not_step_var in H.
 Qed.
 
-
-Lemma In_sty_size_le s phi :
-  In s phi -> sty_size s <= list_sum (map sty_size phi).
+Lemma Admissible_wn : Admissible wn.
 Proof.
-  elim: phi; first done.
-  move=> ?? IH /= [] => [<-|/IH]; lia.
+  constructor.
+  - by apply: head_exp_wn.
+  - by apply: neutal_wn_wn.
+  - by apply: wn_app_var.
 Qed.
 
-Lemma Saturated_interp t : Saturated (fun M => interp M t).
+End Admissible_wn.
+
+(* consequence of fundamental theorem *)
+Lemma weak_normalization Gamma M t : type_assignment Gamma M t -> wn M.
 Proof.
-  elim /(measure_rect sty_size): t. case.
-  { move=> x IH. constructor=> ?.
-    - done.
-    - by apply: head_wn_wn. }
-  move=> s phi t IH. constructor=> M HM /=.
-  - have := HM (var 0).
-    apply: unnest.
-    { split.
-      { have /= := IH s. apply: unnest. { lia. }
-        move=> /Saturated_head_wn. apply. by constructor. }
-      apply /Forall_all /Forall_forall => s' /In_sty_size_le ?.
-      have /= := IH s'. apply: unnest. { lia. }
-      move=> /Saturated_head_wn. apply. by constructor. }
-    have /= := IH t. apply: unnest. { lia. }
-    move=> /Saturated_wn /[apply]. by apply: wn_app_var.
-  - move=> N [+ _].
-    have /= := IH s. apply: unnest. { lia. }
-    move=> /Saturated_wn /[apply] ?.
-    have /= := IH t. apply: unnest. { lia. }
-    move=> /Saturated_head_wn. apply. by constructor.
+  apply: fundamental. by apply: Admissible_wn.Admissible_wn.
 Qed.
-
-Print Assumptions Saturated_interp.
-
-(* this will follow from saturation *)
-Lemma interp_var x t : interp (var x) t.
-Proof.
-  have /Saturated_head_wn := Saturated_interp t.
-  apply. by constructor.
-Qed.
-
-(* this needs interp_var *)
-Lemma interp_wn M t : interp M t -> wn M.
-Proof.
-  have /Saturated_wn := Saturated_interp t. by apply.
-Qed.
-
-Inductive head_red : tm -> tm -> Prop :=
-  | head_red_lam M N : wn N -> head_red (subst (scons N var) M) (app (lam M) N)
-  | head_red_app M M' N : head_red M M' -> wn N -> head_red (app M N) (app M' N).
-
-Lemma head_redE M N : head_red M N ->
-  match N with
-  | app (lam M1) M2 => M = subst (scons M2 var) M1 /\ wn M2
-  | app M1 M2 => exists M', M = app M' M2 /\ head_red M' M1 /\ wn M2
-  | _ => False
-  end.
-Proof.
-  elim. { done. }
-  by move=> ? [] *; [|eexists|].
-Qed.
-
-Lemma head_red_step M N : head_red M N -> step N M.
-Proof.
-  elim. { move=> *. by apply: stepRed. }
-  move=> *. by apply: stepAppL.
-Qed.
-
-Lemma head_red_wn M N : head_red M N -> wn M -> wn N.
-Proof.
-  by move=> /head_red_step /step_wn.
-Qed.
-
-Lemma interp_head_red M N t : head_red M N -> interp M t -> interp N t.
-Proof.
-  elim: t M N.
-  { move=> > ?. by apply: head_red_wn. }
-  move=> s IHs phi t IH M N /= []. rewrite /Arr.
-  - move=> {}M {}N HN IH' ? [Hs ?].
-    apply: IH.
-    { constructor; [by apply: head_red_lam|].
-      have /Saturated_wn := Saturated_interp s. by apply. }
-    by apply: IH'.
-  - move=> > ?? /= IH' ? [??]. apply: IH.
-    { constructor; [constructor|].
-      - eassumption.
-      - done.
-      - have /Saturated_wn := Saturated_interp s. by apply. }
-    by apply: IH'.
-Qed.
-
-(* this will follow from saturation? *)
-Lemma interp_red M N t : wn N -> interp (subst (scons N var) M) t -> interp (app (lam M) N) t.
-Proof.
-  move=> HN. apply: interp_head_red. by apply: head_red_lam.
-Qed.
-
-(* needs stronger positivity assumption for whole derivation ! *)
-Lemma satisI Gamma M t : type_assignment Gamma M t -> satis Gamma M t.
-Proof.
-  elim: M Gamma t.
-  - move=> a > /type_assignmentE [] s phi Ha H.
-    move=> sigma /(_ a _ _ Ha) [] /=.
-    case: H. { by move=> <-. }
-    by move=> + _ /Forall_forall {}H => /H.
-  - move=> ? IH1 ? IH2 ?? /type_assignmentE [] s phi /IH1 {}IH1 /IH2 {}IH3 Hphi.
-    move=> sigma Hsigma /=. apply: (IH1 sigma Hsigma). split.
-    { by apply: IH3. }
-    apply /Forall_all. rewrite -/interp.
-    apply: Forall_impl Hphi => ? /IH2. by apply.
-  - move=> ? IH1 ? [?|s phi t] /type_assignmentE; first done.
-    move=> /IH1 {}IH1 sigma HGamma /=.
-    move=> N [Hs Hphi]. apply: interp_red.
-    { apply: interp_wn. eassumption.  }
-    rewrite simpl_tm. apply: IH1=> - [|i].
-    + move=> /= ?? [<- <-]. by split; [|apply /Forall_all].
-    + move=> ?? /HGamma => - [Hs' Hphi'] /=. by rewrite !simpl_tm.
-Qed.
-
-Lemma weak_normalization Gamma M t : 
-  type_assignment Gamma M t -> wn M.
-Proof.
-  move=> /satisI /(_ var). rewrite simpl_tm.
-  apply: unnest. 
-  { move=> i *. split. { by apply: interp_var. }
-    apply /Forall_forall => *. by apply: interp_var. }
-  by apply: interp_wn.
-Qed.
-
-Print Assumptions weak_normalization.
